@prefix owl: <http://www.w3.org/2002/07/owl#> .
@prefix rdf: <http://www.w3.org/1999/02/22-rdf-syntax-ns#> .
@prefix xml: <http://www.w3.org/XML/1998/namespace> .
@prefix xsd: <http://www.w3.org/2001/XMLSchema#> .
@prefix rdfs: <http://www.w3.org/2000/01/rdf-schema#> .
@prefix movie: <http://example.com/movie#> .
@prefix skos: <http://www.w3.org/2004/02/skos/core#> .

movie:Movie a owl:Class ;
    rdfs:label "Movie" ;
    rdfs:comment "This class represents a movie" ;
    rdfs:subClassOf skos:Concept .

movie:title a owl:DatatypeProperty ;
    rdfs:label "title" ;
    rdfs:comment "This property is for the movie title, it should be a string" ;
    rdfs:domain movie:Movie ;
    rdfs:range xsd:string .

#Cela signifie que si un film a un réalisateur, le réalisateur a réalisé ce film.
movie:Director a owl:ObjectProperty ;
    rdfs:label "director" ;
    rdfs:comment "This property is for the movie's director, it should be a Person" ;
    rdfs:domain movie:Movie ;
    owl:equivalentClass [ owl:intersectionOf ( movie:Person movie:DirectedBy ) ] .

movie:year a owl:DatatypeProperty ;
    rdfs:label "year" ;
    rdfs:comment "This property is for the year the movie was released, it should be a date" ;
    rdfs:domain movie:Movie ;
    rdfs:range xsd:date .

movie:actors a owl:ObjectProperty ;
    rdfs:label "actors" ;
    rdfs:comment "This property is for the movie actors, it should be a list of Person instances" ;
    rdfs:domain movie:Movie ;
    rdfs:range rdf:List .

movie:hasGenre a owl:ObjectProperty ;
    rdfs:label "hasGenre" ;
    rdfs:comment "This property links a movie to its genre" ;
    rdfs:domain movie:Movie ;
    rdfs:range movie:Genre .

movie:Genre a owl:Class ;
    rdfs:label "Genre" ;
    rdfs:comment "This class represents a genre of a movie" ;
    a owl:TransitiveProperty .

movie:genreName a owl:DatatypeProperty ;
    rdfs:label "genreName" ;
    rdfs:comment "This property is for the genre name, it should be a string" ;
    rdfs:domain movie:Genre ;
    rdfs:range xsd:string .

movie:Person a owl:Class ;
    rdfs:label "Person" ;
    rdfs:comment "This class represents a person" .

movie:name a owl:DatatypeProperty ;
    rdfs:label "name" ;
    rdfs:comment "This property is for the person's name, it should be a string" ;
    rdfs:domain movie:Person ;
    rdfs:range xsd:string .

movie:Actor a owl:Class ;
    rdfs:label "Actor" ;
    rdfs:comment "A class representing an actor" ;
    owl:equivalentClass [ owl:intersectionOf ( movie:Person movie:ActsIn ) ] .

movie:ActsIn a owl:ObjectProperty ;
    rdfs:label "ActsIn" ;
    rdfs:comment "An actor acts in a movie" ;
    rdfs:domain movie:Actor ;
    rdfs:range movie:Movie .

movie:DirectedBy a owl:ObjectProperty ;
    rdfs:label "DirectedBy" ;
    rdfs:comment "A movie is directed by a director" ;
    rdfs:domain movie:Movie ;
    rdfs:range movie:Director .

movie:rating a owl:DatatypeProperty ;
    rdfs:label "rating" ;
    rdfs:comment "This property is for the movie rating, it should be a float value" ;
    rdfs:domain movie:Movie ;
    rdfs:range xsd:float .

movie:genres a skos:ConceptScheme;
    skos:hasTopConcept movie:Genre;
    rdfs:label "Movie Genres";
    rdfs:comment "The scheme representing genres of movies" .

movie:Keyword a owl:Class ;
    rdfs:label "Keyword" ;
    rdfs:comment "This class represents a keyword of a movie" .

movie:hasKeyword a owl:ObjectProperty ;
    rdfs:label "hasKeyword" ;
    rdfs:comment "This property is for the movie's keyword, it should be a Keyword instance" ;
    rdfs:domain movie:Movie ;
    rdfs:range movie:Keyword .

movie:relatedTo a owl:ObjectProperty ;
    rdfs:label "relatedTo" ;
    rdfs:comment "This property links a movie to other related movies" ;
    rdfs:domain movie:Movie ;
    rdfs:range movie:Movie .

movie:ActorName a owl:DatatypeProperty ;
    rdfs:label "ActorName" ;
    rdfs:comment "This property is for the actor name, it should be a string" ;
    rdfs:domain movie:Actor ;
    rdfs:range xsd:string .

movie:ActorRole a owl:DatatypeProperty ;
    rdfs:label "ActorRole" ;
    rdfs:comment "This property is for the actor role, it should be a string" ;
    rdfs:domain movie:Actor ;
    rdfs:range xsd:string .

movie:Adult a owl:DatatypeProperty ;
    rdfs:label "Adult" ;
    rdfs:comment "This property is for the adult content, it should be a boolean" ;
    rdfs:domain movie:Movie ;
    rdfs:range xsd:boolean .

movie:OriginalLanguage a owl:DatatypeProperty ;
    rdfs:label "OriginalLanguage" ;
    rdfs:comment "This property is for the original language of the movie, it should be a string" ;
    rdfs:domain movie:Movie ;
    rdfs:range xsd:string .

movie:OriginalTitle a owl:DatatypeProperty ;
    rdfs:label "OriginalTitle" ;
    rdfs:comment "This property is for the original title of the movie, it should be a string" ;
    rdfs:domain movie:Movie ;
    rdfs:range xsd:string .

movie:Overview a owl:DatatypeProperty ;
    rdfs:label "Overview" ;
    rdfs:comment "This property is for the overview of the movie, it should be a string" ;
    rdfs:domain movie:Movie ;
    rdfs:range xsd:string .

movie:Popularity a owl:DatatypeProperty ;
    rdfs:label "Popularity" ;
    rdfs:comment "This property is for the popularity of the movie, it should be a double" ;
    rdfs:domain movie:Movie ;
    rdfs:range xsd:double .

movie:PosterPath a owl:DatatypeProperty ;
    rdfs:label "PosterPath" ;
    rdfs:comment "This property is for the path of the poster of the movie, it should be a string" ;
    rdfs:domain movie:Movie ;
    rdfs:range xsd:string .

movie:Video a owl:DatatypeProperty ;
    rdfs:label "Video" ;
    rdfs:comment "This property is for the availability of the video, it should be a boolean" ;
    rdfs:domain movie:Movie ;
    rdfs:range xsd:boolean .

movie:VoteAverage a owl:DatatypeProperty ;
    rdfs:label "VoteAverage" ;
    rdfs:comment "This property is for the average vote of the movie, it should be a double" ;
    rdfs:domain movie:Movie ;
    rdfs:range xsd:double .

movie:VoteCount a owl:DatatypeProperty ;
    rdfs:label "VoteCount" ;
    rdfs:comment "This property is for the number of votes of the movie, it should be an integer" ;
    rdfs:domain movie:Movie ;
    rdfs:range xsd:integer .

movie:hasGenre a owl:ObjectProperty ;
    rdfs:label "hasGenre" ;
    rdfs:comment "This property is for the genres of the movie, it should be an object" ;
    rdfs:domain movie:Movie ;
    rdfs:range <http://myvocab.org/genre/> .

movie:duration a owl:DatatypeProperty ;
    rdfs:label "duration" ;
    rdfs:range xsd:decimal .

movie:LongMovie a owl:Class ;
    rdfs:label "Long Movie" ;
    rdfs:subClassOf movie:Movie .

movie:LongMovieDurationRestriction a owl:Restriction ;
    owl:onProperty movie:duration ;
    owl:minInclusive "120"^^xsd:decimal .

movie:LongMovie rdfs:subClassOf movie:LongMovieDurationRestriction .
